separate traces and validity

src/Transition.v
@@ -49,146 +49,248 @@ Section Protocols.
   Definition transition_dec p :=
     forall q : p.(state), {q' : p.(state) & state_lt q' q} + {final q}.
 
-  (* TODO use more traditional semantics style than these traces *)
+  Inductive trace p : Type :=
+  | TInitial : p.(state) -> trace p
+  | TTransition : p.(state) -> trace p -> trace p.
 
-  Inductive reaches p : p.(state) -> Type :=
-  | RInitial : reaches p.(initial)
-  | RTransition : forall q q' (t : state_lt q' q),
-                    reaches q -> reaches q'.
+  Definition head p (tr : trace p) := match tr with
+                                        | TInitial q => q
+                                        | TTransition q _ => q
+                                      end.
 
-  Fixpoint reaches_n p (q : p.(state)) (R : reaches q) : nat :=
-    match R with
-      | RInitial _ => O
-      | @RTransition _ q' _ _ R => S (@reaches_n p q' R)
+  Fixpoint tr_len p (tr : trace p) :=
+    match tr with
+      | TInitial _ => 0
+      | TTransition _ tr => S (tr_len tr)
     end.
 
-  Lemma root_unique p (q : p.(state)) (R : reaches q) :
-    reaches_n R = 0 -> q = p.(initial).
+  Inductive valid p : trace p -> Prop :=
+  | VInitial : valid (TInitial p.(initial))
+  | VTransition : forall q' (tr : trace p) (t : state_lt q' (head tr)),
+                    valid tr -> valid (TTransition q' tr).
+
+  Definition complete p (tr : trace p) := final (head tr).
+
+   (* Definition Trace p := sigT (@valid p). *)
+
+  (* Definition proj_tr p : Trace p -> trace p := @projT1 _ (@valid p). *)
+
+  (* Definition Tr_len p (R : Trace p) : nat := tr_len (proj_tr R). *)
+
+  Lemma trace_root_unique p (R : trace p) (vR : valid R) :
+    tr_len R = 0 -> R = (TInitial p.(initial)).
     intro H.
-    induction R.
+    induction vR.
     reflexivity.
-    simpl in H; discriminate.
+    inversion H.
   Qed.
 
-  Lemma reaches_n_inv p (q : p.(state)) (R : reaches q) n :
-    reaches_n R = S n ->
-    exists q' (t : state_lt q q') (R' : reaches q'),
-      R = (RTransition t R') /\ reaches_n R' = n.
-    intro H.
-    revert n H.
+  Definition tr_len_inv p (R : trace p) n :
+    tr_len R = S n ->
+    {q' : p.(state) &
+          {R' : trace p | R = (TTransition q' R') /\ tr_len R' = n}}.
+    revert n.
     remember R as r.
-    destruct r as [| q' q H0 r]; intros n H.
+    destruct r as [| q' r]; intros n H.
     inversion H.
 
     exists q'.
-    exists H0.
     exists r.
     split.
     reflexivity.
 
     inversion H.
     reflexivity.
+ Defined.
+
+  Lemma valid_inv p (q' : p.(state)) (R : trace p)
+        (vRt : valid (TTransition q' R)) : valid R.
+    inversion vRt.
+    assumption.
   Qed.
 
-  Lemma reaches_unique_n p (U : unique_transition p) (q q' : p.(state))
-        (R : reaches q) (R' : reaches q') :
-    reaches_n R = reaches_n R' -> q = q'.
-    remember (reaches_n R) as n eqn:HnR.
+  Definition valid_len_inv p (R : trace p) (vR : valid R) n :
+    tr_len R = S n ->
+    {q : p.(state) &
+         {R' : trace p | R = (TTransition q R') /\ tr_len R' = n /\
+                         valid R'}}.
+    intro H.
+    destruct (tr_len_inv H) as [q' [R' [eR' en]]].
+    exists q'.
+    exists R'.
+    split; [|split]; [assumption ..|].
+    subst R.
+    eapply valid_inv; eassumption.
+  Defined.
+
+  Lemma unique_valid_extension p (U : unique_transition p)
+        (R : trace p) (q q' : p.(state))
+        (vRq : valid (TTransition q R)) (vRq' : valid (TTransition q' R)) :
+    q = q'.
+    inversion vRq.
+    inversion vRq'.
+    eapply U.
+    eassumption.
+    eassumption.
+  Qed.
+
+  Lemma trace_unique_n p (U : unique_transition p)
+        (R R' : trace p) (vR : valid R) (vR' : valid R') :
+    tr_len R = tr_len R' -> R = R'.
+    remember (tr_len R) as n eqn:HnR.
     intro HnR'.
     symmetry in HnR, HnR'.
-    revert q q' R R' HnR HnR'.
-    induction n; intros q q' R R' HnR HnR'.
-    assert (q = p.(initial)) by (eapply root_unique; eassumption); subst q.
-    assert (q' = p.(initial)) by (eapply root_unique; eassumption); subst q'.
+    revert R R' vR vR' HnR HnR'.
+    induction n; intros R R' vR vR' HnR HnR'.
+    assert (R = TInitial p.(initial)) by
+        (eapply trace_root_unique; eassumption); subst R.
+    assert (R' = TInitial p.(initial)) by
+        (eapply trace_root_unique; eassumption); subst R'.
     reflexivity.
-    pose proof (reaches_n_inv HnR) as H.
-    pose proof (reaches_n_inv HnR') as H'.
+
+    pose proof (valid_len_inv vR HnR) as H.
+    pose proof (valid_len_inv vR' HnR') as H'.
     clear HnR HnR'.
-    destruct H as [q0 [? [? [? ?]]]].
+    destruct H as [q0 [R0 [? [? ?]]]].
     subst R.
 
-    destruct H' as [q0' [? [? [? ?]]]].
+    destruct H' as [q'0 [R'0 [? [? ?]]]].
     subst R'.
 
-    assert (q0 = q0') by (eapply IHn; eassumption).
-    subst q0'.
+    assert (R0 = R'0) by (eapply IHn; eassumption); subst R'0.
 
-    eapply U; eassumption.
+    assert (q0 = q'0) by (eapply unique_valid_extension; eassumption);
+      subst q'0.
+
+    reflexivity.
   Qed.
 
-  Lemma no_final_greater p (U : unique_transition p) (q q' : p.(state))
-        (R : reaches q) (R' : reaches q') :
-    final q -> reaches_n R < reaches_n R' -> False.
-    intros Fq l.
+  Lemma complete_no_extension p (q : p.(state)) (R : trace p) :
+    (complete R) -> valid (TTransition q R) -> False.
+    intros cR vRq.
+    inversion vRq.
+    eapply cR; eassumption.
+  Qed.
 
-    assert (exists n, reaches_n R' = S (n + reaches_n R)) as l' by
-          (exists (reaches_n R' - reaches_n R - 1); omega); clear l.
+  Lemma complete_no_greater p (U : unique_transition p)
+        (R R' : trace p) (vR : valid R) (vR' : valid R') :
+    complete R -> tr_len R < tr_len R' -> False.
+    intros cR l.
+
+    assert (exists n, tr_len R' = S (n + tr_len R)) as l' by
+          (exists (tr_len R' - tr_len R - 1); omega); clear l.
     destruct l' as [n H].
-    destruct (reaches_n_inv H) as [q'0 [t'0 [R'0 [_ HnR'0]]]]; clear H R'.
+    destruct (valid_len_inv vR' H) as [q'0 [R'0 [? [HnR'0 vR'0]]]];
+      clear H; subst R'.
 
-    revert q' q'0 t'0 R'0 HnR'0.
-    induction n; intros q' q'0 t'0 R'0 HnR'0.
+    revert q'0 R'0 HnR'0 vR' vR'0.
+    induction n; intros q'0 R'0 HnR'0 vR' vR'0.
 
     simpl in HnR'0.
-    assert (q = q'0) by
-        (symmetry in HnR'0; eapply reaches_unique_n; eassumption).
-    subst q'0.
-    eapply Fq; eassumption.
+    assert (R = R'0) by
+        (symmetry in HnR'0; eapply trace_unique_n; eassumption); subst R'0.
+    eapply complete_no_extension; eassumption.
 
-    destruct (reaches_n_inv HnR'0) as [q'1 [t'1 [R'1 [_ HnR'1]]]].
-    clear HnR'0 R'0.
+    destruct (valid_len_inv vR'0 HnR'0) as [q'1 [R'1 [? [HnR'1 vR'1]]]];
+      clear HnR'0; subst R'0.
 
     eapply IHn; swap 1 2; eassumption.
   Qed.
 
-  Lemma reaches_unique_final_n p (U : unique_transition p)
-        (q q' : p.(state)) (R : reaches q)
-        (R' : reaches q') :
-    final q -> final q' -> reaches_n R = reaches_n R'.
-    intros Fq Fq'.
-    destruct (lt_eq_lt_dec (reaches_n R) (reaches_n R')) as [[l | e] | l];
+  Lemma complete_same_len p (U : unique_transition p)
+        (R : trace p) (R' : trace p) :
+    valid R -> valid R' -> complete R -> complete R' -> tr_len R = tr_len R'.
+    intros.
+    destruct (lt_eq_lt_dec (tr_len R) (tr_len R')) as [[l | e] | l];
       [exfalso | assumption | exfalso];
-      eapply no_final_greater; swap 2 3; eassumption.
+      [ > eapply complete_no_greater; swap 1 5 .. ]; eassumption.
   Qed.
 
-  Theorem reaches_unique_final p (U : unique_transition p) (q q' : p.(state))
-          (R : reaches q) (R' : reaches q') :
-    final q -> final q' -> q = q'.
-    intros Fq Fq'.
-    eapply reaches_unique_n with (R := R) (R' := R');
-      [assumption | eapply reaches_unique_final_n; eassumption].
+  Theorem complete_unique p (U : unique_transition p)
+          (R : trace p) (R' : trace p) :
+    valid R -> valid R' -> complete R -> complete R' -> R = R'.
+    intros.
+    eapply trace_unique_n with (R := R) (R' := R');
+      try eapply complete_same_len; eassumption.
   Qed.
 
-
-  Definition extend_reach p (E : transition_dec p) (q : p.(state))
-             (R : reaches q) :
-    {q' : p.(state) & (reaches q') * state_lt q' q}%type + {final q}.
-    destruct (E q) as [[q' t] | Fq].
-    left; exists q'; split; [econstructor|]; eassumption.
+  Definition extend_trace p (E : transition_dec p)
+             (R : trace p) (vR : valid R) :
+    {R' : trace p | valid R' /\ state_lt (head R') (head R)}%type +
+    {complete R}.
+    destruct (E (head R)) as [[q' t] | Fq].
+    left; eexists; split; [econstructor|]; eassumption.
     right; assumption.
   Defined.
 
-  Definition finalize_reach p (E : transition_dec p) (q : p.(state))
-             (R : reaches q) :
-    {q' : p.(state) & (reaches q') * (final q')}%type.
-    revert q R.
-    refine
-      (Fix p.(@state_wf)
-               (fun q : p.(state) =>
-                  reaches (p:=p) q ->
-                  {q' : state p &
-                        (reaches (p:=p) q' * final (p:=p) q')%type}) _).
-    intros q IHq R.
-    destruct (E q) as [[q' t] | Fq].
-    eapply IHq; [|econstructor]; eassumption.
+  Definition tr_lt p (R R' : trace p) : Prop := state_lt (head R) (head R').
 
-    exists q.
-    split; assumption.
+  Fixpoint tr_with_head_tail p (q : p.(state)) qs :=
+    match qs with
+      | [] => TInitial q
+      | q' :: qs' => TTransition q (tr_with_head_tail q' qs')
+    end.
+
+  Fixpoint tail p (R : trace p) : list p.(state) :=
+    match R with
+      | TInitial _ => []
+      | TTransition _ R => head R :: tail R
+    end.
+
+  Lemma head_tail_inv p (R : trace p) :
+    R = tr_with_head_tail (head R) (tail R).
+    induction R.
+    reflexivity.
+    simpl.
+    rewrite IHR at 1.
+    reflexivity.
+  Qed.
+
+  Lemma head_inv p (q : p.(state)) qs :
+    q = head (tr_with_head_tail (p:=p) q qs).
+    induction qs; reflexivity.
+  Qed.
+
+  Definition tr_wf p : well_founded (@tr_lt p).
+    unfold well_founded.
+    intro R.
+    rewrite head_tail_inv.
+
+    refine ((Fix p.(@state_wf)
+                     (fun q => forall R, Acc (tr_lt (p:=p))
+                                             (tr_with_head_tail q (tail R)))
+                     _ _) R); clear R.
+
+    intros q IHq Rtl.
+    constructor.
+    intros R' H.
+    unfold tr_lt in H.
+    rewrite <- head_inv in H.
+    specialize (IHq (head R') H R').
+    rewrite <- head_tail_inv in IHq.
+    assumption.
   Defined.
 
-  Definition exists_reaches p (E : transition_dec p) :
-    {q : p.(state) & (reaches q) * (final q)}%type.
-    eapply finalize_reach; [assumption | constructor].
+  Definition finalize_trace p (E : transition_dec p)
+             (R : trace p) (vR : valid R) :
+    {R' : trace p | valid R' /\ complete R'}%type.
+    revert R vR.
+    refine
+      (Fix (@tr_wf p)
+           (fun R : trace p =>
+              valid R ->
+              {R' : trace p | valid R' /\ complete R'}) _).
+    intros R IHR vR.
+    destruct (extend_trace E vR) as [[R' [vR' t]] | cR].
+
+    eapply IHR; eassumption.
+
+    exists R; split; assumption.
+  Defined.
+
+  Definition exists_trace p (E : transition_dec p) :
+    {R : trace p | valid R /\ complete R}%type.
+    eapply finalize_trace; [assumption | constructor].
   Defined.
 
 End Protocols.
